doc: documentation for Init.Core

src/Init/Core.lean
@@ -8,11 +8,23 @@ notation, basic datatypes and type classes
 prelude
 import Init.Prelude
 import Init.SizeOf
+set_option linter.missingDocs true -- keep it documented
 
 universe u v w
 
+/--
+`inline f x` is an indication to the compiler to inline the definition of `f`
+at the application site itself (by comparison to the `@[inline]` attribute,
+which applies to all applications of the function).
+-/
 def inline {α : Sort u} (a : α) : α := a
 
+/--
+`flip f a b` is `f b a`. It is useful for "point-free" programming,
+since it can sometimes be used to avoid introducing variables.
+For example, `(·<·)` is the less-than relation,
+and `flip (·<·)` is the greater-than relation.
+-/
 @[inline] def flip {α : Sort u} {β : Sort v} {φ : Sort w} (f : α → β → φ) : β → α → φ :=
   fun b a => f a b
 
@@ -27,6 +39,10 @@ attribute [simp] namedPattern
   The value is then stored and not recomputed for all further accesses. -/
 -- NOTE: the runtime has special support for the `Thunk` type to implement this behavior
 structure Thunk (α : Type u) : Type u where
+  /-- Constructs a new thunk from a function `Unit → α`
+  that will be called when the thunk is forced. -/
+  mk ::
+  /-- Extract the getter function out of a thunk. Use `Thunk.get` instead. -/
   private fn : Unit → α
 
 attribute [extern "lean_mk_thunk"] Thunk.mk
@@ -34,105 +50,317 @@ attribute [extern "lean_mk_thunk"] Thunk.mk
 /-- Store a value in a thunk. Note that the value has already been computed, so there is no laziness. -/
 @[extern "lean_thunk_pure"] protected def Thunk.pure (a : α) : Thunk α :=
   ⟨fun _ => a⟩
+
+/--
+Forces a thunk to extract the value. This will cache the result,
+so a second call to the same function will return the value in O(1)
+instead of calling the stored getter function.
+-/
 -- NOTE: we use `Thunk.get` instead of `Thunk.fn` as the accessor primitive as the latter has an additional `Unit` argument
 @[extern "lean_thunk_get_own"] protected def Thunk.get (x : @& Thunk α) : α :=
   x.fn ()
+
+/-- Map a function over a thunk. -/
 @[inline] protected def Thunk.map (f : α → β) (x : Thunk α) : Thunk β :=
   ⟨fun _ => f x.get⟩
+/-- Constructs a thunk that applies `f` to the result of `x` when forced. -/
 @[inline] protected def Thunk.bind (x : Thunk α) (f : α → Thunk β) : Thunk β :=
   ⟨fun _ => (f x.get).get⟩
 
 @[simp] theorem Thunk.sizeOf_eq [SizeOf α] (a : Thunk α) : sizeOf a = 1 + sizeOf a.get := by
    cases a; rfl
 
+/-- A variation on `Eq.ndrec` with the equality argument first. -/
 abbrev Eq.ndrecOn.{u1, u2} {α : Sort u2} {a : α} {motive : α → Sort u1} {b : α} (h : a = b) (m : motive a) : motive b :=
   Eq.ndrec m h
 
+/--
+If and only if, or logical bi-implication. `a ↔ b` means that `a` implies `b` and vice versa.
+By `propext`, this implies that `a` and `b` are equal and hence any expression involving `a`
+is equivalent to the corresponding expression with `b` instead.
+-/
 structure Iff (a b : Prop) : Prop where
-  intro :: (mp : a → b) (mpr : b → a)
+  /-- If `a → b` and `b → a` then `a` and `b` are equivalent. -/
+  intro ::
+  /-- Modus ponens for if and only if. If `a ↔ b` and `a`, then `b`. -/
+  mp : a → b
+  /-- Modus ponens for if and only if, reversed. If `a ↔ b` and `b`, then `a`. -/
+  mpr : b → a
 
-infix:20 " <-> " => Iff
-infix:20 " ↔ "   => Iff
+@[inheritDoc] infix:20 " <-> " => Iff
+@[inheritDoc] infix:20 " ↔ "   => Iff
 
+/--
+`Sum α β`, or `α ⊕ β`, is the disjoint union of types `α` and `β`.
+An element of `α ⊕ β` is either of the form `.inl a` where `a : α`,
+or `.inr b` where `b : β`.
+-/
 inductive Sum (α : Type u) (β : Type v) where
-  | inl (val : α) : Sum α β
-  | inr (val : β) : Sum α β
+  | /-- Left injection into the sum type `α ⊕ β`. If `a : α` then `.inl a : α ⊕ β`. -/
+    inl (val : α) : Sum α β
+  | /-- Right injection into the sum type `α ⊕ β`. If `b : β` then `.inr b : α ⊕ β`. -/
+    inr (val : β) : Sum α β
 
-infixr:30 " ⊕ " => Sum
+@[inheritDoc] infixr:30 " ⊕ " => Sum
 
+/--
+`PSum α β`, or `α ⊕' β`, is the disjoint union of types `α` and `β`.
+It differs from `α ⊕ β` in that it allows `α` and `β` to have arbitrary sorts
+`Sort u` and `Sort v`, instead of restricting to `Type u` and `Type v`. This means
+that it can be used in situations where one side is a proposition, like `True ⊕' Nat`.
+
+The reason this is not the default is that this type lives in the universe `Sort (max 1 u v)`,
+which can cause problems for universe level unification,
+because the equation `max 1 u v = ?u + 1` has no solution in level arithmetic.
+`PSum` is usually only used in automation that constructs sums of arbitrary types.
+-/
 inductive PSum (α : Sort u) (β : Sort v) where
-  | inl (val : α) : PSum α β
-  | inr (val : β) : PSum α β
+  | /-- Left injection into the sum type `α ⊕' β`. If `a : α` then `.inl a : α ⊕' β`. -/
+    inl (val : α) : PSum α β
+  | /-- Right injection into the sum type `α ⊕' β`. If `b : β` then `.inr b : α ⊕' β`. -/
+    inr (val : β) : PSum α β
 
-infixr:30 " ⊕' " => PSum
+@[inheritDoc] infixr:30 " ⊕' " => PSum
 
+/--
+`Sigma β`, also denoted `Σ a : α, β a` or `(a : α) × β a`, is the type of dependent pairs
+whose first component is `a : α` and whose second component is `b : β a`
+(so the type of the second component can depend on the value of the first component).
+It is sometimes known as the dependent sum type, since it is the type level version
+of an indexed summation.
+-/
 structure Sigma {α : Type u} (β : α → Type v) where
+  /-- Constructor for a dependent pair. If `a : α` and `b : β a` then `⟨a, b⟩ : Sigma β`.
+  (This will usually require a type ascription to determine `β`
+  since it is not determined from `a` and `b` alone.) -/
+  mk ::
+  /-- The first component of a dependent pair. If `p : @Sigma α β` then `p.1 : α`. -/
   fst : α
+  /-- The second component of a dependent pair. If `p : Sigma β` then `p.2 : β p.1`. -/
   snd : β fst
 
 attribute [unbox] Sigma
 
+/--
+`PSigma β`, also denoted `Σ' a : α, β a` or `(a : α) ×' β a`, is the type of dependent pairs
+whose first component is `a : α` and whose second component is `b : β a`
+(so the type of the second component can depend on the value of the first component).
+It differs from `Σ a : α, β a` in that it allows `α` and `β` to have arbitrary sorts
+`Sort u` and `Sort v`, instead of restricting to `Type u` and `Type v`. This means
+that it can be used in situations where one side is a proposition, like `(p : Nat) ×' p = p`.
+
+The reason this is not the default is that this type lives in the universe `Sort (max 1 u v)`,
+which can cause problems for universe level unification,
+because the equation `max 1 u v = ?u + 1` has no solution in level arithmetic.
+`PSigma` is usually only used in automation that constructs pairs of arbitrary types.
+-/
 structure PSigma {α : Sort u} (β : α → Sort v) where
+  /-- Constructor for a dependent pair. If `a : α` and `b : β a` then `⟨a, b⟩ : PSigma β`.
+  (This will usually require a type ascription to determine `β`
+  since it is not determined from `a` and `b` alone.) -/
+  mk ::
+  /-- The first component of a dependent pair. If `p : @Sigma α β` then `p.1 : α`. -/
   fst : α
+  /-- The second component of a dependent pair. If `p : Sigma β` then `p.2 : β p.1`. -/
   snd : β fst
 
-inductive Exists {α : Sort u} (p : α → Prop) : Prop where
-  | intro (w : α) (h : p w) : Exists p
+/--
+Existential quantification. If `p : α → Prop` is a predicate, then `∃ x : α, p x`
+asserts that there is some `x` of type `α` such that `p x` holds.
+To create an existential proof, use the `exists` tactic,
+or the anonymous constructor notation `⟨x, h⟩`.
+To unpack an existential, use `cases h` where `h` is a proof of `∃ x : α, p x`,
+or `let ⟨x, hx⟩ := h` where `.
 
-/-- Auxiliary type used to compile `for x in xs` notation. -/
+Because Lean has proof irrelevance, any two proofs of an existential are
+definitionally equal. One consequence of this is that it is impossible to recover the
+witness of an existential from the mere fact of its existence.
+For example, the following does not compile:
+```
+example (h : ∃ x : Nat, x = x) : Nat :=
+  let ⟨x, _⟩ := h  -- fail, because the goal is `Nat : Type`
+  x
+```
+The error message `recursor 'Exists.casesOn' can only eliminate into Prop` means
+that this only works when the current goal is another proposition:
+```
+example (h : ∃ x : Nat, x = x) : True :=
+  let ⟨x, _⟩ := h  -- ok, because the goal is `True : Prop`
+  trivial
+```
+-/
+inductive Exists {α : Sort u} (p : α → Prop) : Prop where
+  | /-- Existential introduction. If `a : α` and `h : p a`,
+    then `⟨a, h⟩` is a proof that `∃ x : α, p x`. -/
+    intro (w : α) (h : p w) : Exists p
+
+/--
+Auxiliary type used to compile `for x in xs` notation.
+
+This is the return value of the body of a `ForIn` call,
+representing the body of a for loop. It can be:
+
+* `.yield (a : α)`, meaning that we should continue the loop and `a` is the new state.
+  `.yield` is produced by `continue` and reaching the bottom of the loop body.
+* `.done (a : α)`, meaning that we should early-exit the loop with state `a`.
+  `.done` is produced by calls to `break` or `return` in the loop,
+-/
 inductive ForInStep (α : Type u) where
-  | done  : α → ForInStep α
-  | yield : α → ForInStep α
+  | /-- `.done a` means that we should early-exit the loop.
+    `.done` is produced by calls to `break` or `return` in the loop. -/
+    done  : α → ForInStep α
+  | /-- `.yield a` means that we should continue the loop.
+    `.yield` is produced by `continue` and reaching the bottom of the loop body. -/
+    yield : α → ForInStep α
   deriving Inhabited
 
+/--
+`ForIn m ρ α` is the typeclass which supports `for x in xs` notation.
+Here `xs : ρ` is the type of the collection to iterate over, `x : α`
+is the element type which is made available inside the loop, and `m` is the monad
+for the encompassing `do` block.
+-/
 class ForIn (m : Type u₁ → Type u₂) (ρ : Type u) (α : outParam (Type v)) where
+  /-- `forIn x b f : m β` runs a for-loop in the monad `m` with additional state `β`.
+  This traverses over the "contents" of `x`, and passes the elements `a : α` to
+  `f : α → β → m (ForInStep β)`. `b : β` is the initial state, and the return value
+  of `f` is the new state as well as a directive `.done` or `.yield`
+  which indicates whether to abort early or continue iteration.
+
+  The expression
+  ```
+  let mut b := ...
+  for x in xs do
+    b ← foo x b
+  ```
+  in a `do` block is syntactic sugar for:
+  ```
+  let b := ...
+  let b ← forIn xs b (fun x b => do
+    let b ← foo x b
+    return .yield b)
+  ```
+  (Here `b` corresponds to the variables mutated in the loop.) -/
   forIn {β} [Monad m] (x : ρ) (b : β) (f : α → β → m (ForInStep β)) : m β
 
 export ForIn (forIn)
 
+/--
+`ForIn' m ρ α d` is a variation on the `ForIn m ρ α` typeclass which supports the
+`for h : x in xs` notation. It is the same as `for x in xs` except that `h : x ∈ xs`
+is provided as an additional argument to the body of the for-loop.
+-/
 class ForIn' (m : Type u₁ → Type u₂) (ρ : Type u) (α : outParam (Type v)) (d : outParam $ Membership α ρ) where
+  /-- `forIn' x b f : m β` runs a for-loop in the monad `m` with additional state `β`.
+  This traverses over the "contents" of `x`, and passes the elements `a : α` along
+  with a proof that `a ∈ x` to `f : (a : α) → a ∈ x → β → m (ForInStep β)`.
+  `b : β` is the initial state, and the return value
+  of `f` is the new state as well as a directive `.done` or `.yield`
+  which indicates whether to abort early or continue iteration. -/
   forIn' {β} [Monad m] (x : ρ) (b : β) (f : (a : α) → a ∈ x → β → m (ForInStep β)) : m β
 
 export ForIn' (forIn')
 
 
-/-- Auxiliary type used to compile `do` notation. -/
+/--
+Auxiliary type used to compile `do` notation. It is used when compiling a do block
+nested inside a combinator like `tryCatch`. It encodes the possible ways the
+block can exit:
+* `pure (a : α) s` means that the block exited normally with return value `a`.
+* `return (b : β) s` means that the block exited via a `return b` early-exit command.
+* `break s` means that `break` was called, meaning that we should exit
+  from the containing loop.
+* `continue s` means that `continue` was called, meaning that we should continue
+  to the next iteration of the containing loop.
+
+All cases return a value `s : σ` which bundles all the mutable variables of the do-block.
+-/
 inductive DoResultPRBC (α β σ : Type u) where
-  | pure     : α → σ → DoResultPRBC α β σ
-  | return   : β → σ → DoResultPRBC α β σ
-  | break    : σ → DoResultPRBC α β σ
-  | continue : σ → DoResultPRBC α β σ
+  | /-- `pure (a : α) s` means that the block exited normally with return value `a` -/
+    pure : α → σ → DoResultPRBC α β σ
+  | /-- `return (b : β) s` means that the block exited via a `return b` early-exit command -/
+    return : β → σ → DoResultPRBC α β σ
+  | /-- `break s` means that `break` was called, meaning that we should exit
+    from the containing loop -/
+    break : σ → DoResultPRBC α β σ
+  | /-- `continue s` means that `continue` was called, meaning that we should continue
+    to the next iteration of the containing loop -/
+    continue : σ → DoResultPRBC α β σ
 
-/-- Auxiliary type used to compile `do` notation. -/
+/--
+Auxiliary type used to compile `do` notation. It is the same as
+`DoResultPRBC α β σ` except that `break` and `continue` are not available
+because we are not in a loop context.
+-/
 inductive DoResultPR (α β σ : Type u) where
-  | pure   : α → σ → DoResultPR α β σ
-  | return : β → σ → DoResultPR α β σ
+  | /-- `pure (a : α) s` means that the block exited normally with return value `a` -/
+    pure   : α → σ → DoResultPR α β σ
+  | /-- `return (b : β) s` means that the block exited via a `return b` early-exit command -/
+    return : β → σ → DoResultPR α β σ
 
-/-- Auxiliary type used to compile `do` notation. -/
+/--
+Auxiliary type used to compile `do` notation. It is an optimization of
+`DoResultPRBC PEmpty PEmpty σ` to remove the impossible cases,
+used when neither `pure` nor `return` are possible exit paths.
+-/
 inductive DoResultBC (σ : Type u) where
-  | break    : σ → DoResultBC σ
-  | continue : σ → DoResultBC σ
+  | /-- `break s` means that `break` was called, meaning that we should exit
+    from the containing loop -/
+    break    : σ → DoResultBC σ
+  | /-- `continue s` means that `continue` was called, meaning that we should continue
+    to the next iteration of the containing loop -/
+    continue : σ → DoResultBC σ
 
-/-- Auxiliary type used to compile `do` notation. -/
+/--
+Auxiliary type used to compile `do` notation. It is an optimization of
+either `DoResultPRBC α PEmpty σ` or `DoResultPRBC PEmpty α σ` to remove the
+impossible case, used when either `pure` or `return` is never used.
+-/
 inductive DoResultSBC (α σ : Type u) where
-  | pureReturn : α → σ → DoResultSBC α σ
-  | break      : σ → DoResultSBC α σ
-  | continue   : σ → DoResultSBC α σ
+  | /-- This encodes either `pure (a : α)` or `return (a : α)`:
+    * `pure (a : α) s` means that the block exited normally with return value `a`
+    * `return (b : β) s` means that the block exited via a `return b` early-exit command
 
-class HasEquiv  (α : Sort u) where
+    The one that is actually encoded depends on the context of use. -/
+    pureReturn : α → σ → DoResultSBC α σ
+  | /-- `break s` means that `break` was called, meaning that we should exit
+    from the containing loop -/
+    break    : σ → DoResultSBC α σ
+  | /-- `continue s` means that `continue` was called, meaning that we should continue
+    to the next iteration of the containing loop -/
+    continue   : σ → DoResultSBC α σ
+
+/-- `HasEquiv α` is the typeclass which supports the notation `x ≈ y` where `x y : α`.-/
+class HasEquiv (α : Sort u) where
+  /-- `x ≈ y` says that `x` and `y` are equivalent. Because this is a typeclass,
+  the notion of equivalence is type-dependent. -/
   Equiv : α → α → Sort v
 
-infix:50 " ≈ "  => HasEquiv.Equiv
+@[inheritDoc] infix:50 " ≈ "  => HasEquiv.Equiv
 
+/-- `EmptyCollection α` is the typeclass which supports the notation `∅`, also written as `{}`. -/
 class EmptyCollection (α : Type u) where
+  /-- `∅` or `{}` is the empty set or empty collection.
+  It is supported by the `EmptyCollection` typeclass. -/
   emptyCollection : α
 
-notation "{" "}" => EmptyCollection.emptyCollection
-notation "∅"     => EmptyCollection.emptyCollection
+@[inheritDoc] notation "{" "}" => EmptyCollection.emptyCollection
+@[inheritDoc] notation "∅"     => EmptyCollection.emptyCollection
 
-/-- Remark: tasks have an efficient implementation in the runtime. -/
+/--
+`Task α` is a primitive for asynchronous computation.
+It represents a computation that will resolve to a value of type `α`,
+possibly being computed on another thread. This is similar to `Future` in Scala,
+`Promise` in Javascript, and `JoinHandle` in Rust.
+
+The tasks have an overridden representation in the runtime.
+-/
 structure Task (α : Type u) : Type u where
-  pure :: (get : α)
+  /-- `Task.pure (a : α)` constructs a task that is already resolved with value `a`. -/
+  pure ::
+  /-- If `task : Task α` then `task.get : α` blocks the current thread until the
+  value is available, and then returns the result of the task. -/
+  get : α
   deriving Inhabited
 
 attribute [extern "lean_task_pure"] Task.pure
@@ -141,39 +369,86 @@ attribute [extern "lean_task_get_own"] Task.get
 namespace Task
 /-- Task priority. Tasks with higher priority will always be scheduled before ones with lower priority. -/
 abbrev Priority := Nat
+
+/-- The default priority for spawned tasks, also the lowest priority: `0`. -/
 def Priority.default : Priority := 0
+/--
+The highest regular priority for spawned tasks: `8`.
+
+Spawning a task with a priority higher than `Task.Priority.max` is not an error but
+will spawn a dedicated worker for the task, see `Task.Priority.dedicated`.
+Regular priority tasks are placed in a thread pool and worked on according to the priority order.
+-/
 -- see `LEAN_MAX_PRIO`
 def Priority.max : Priority := 8
 /--
-  Any priority higher than `Task.Priority.max` will result in the task being scheduled immediately on a dedicated thread.
-  This is particularly useful for long-running and/or I/O-bound tasks since Lean will by default allocate no more
-  non-dedicated workers than the number of cores to reduce context switches. -/
+Any priority higher than `Task.Priority.max` will result in the task being scheduled
+immediately on a dedicated thread. This is particularly useful for long-running and/or
+I/O-bound tasks since Lean will by default allocate no more non-dedicated workers
+than the number of cores to reduce context switches.
+-/
 def Priority.dedicated : Priority := 9
 
 set_option linter.unusedVariables.funArgs false in
+/--
+`spawn fn : Task α` constructs and immediately launches a new task for
+evaluating the function `fn () : α` asynchronously.
+
+`prio`, if provided, is the priority of the task.
+-/
 @[noinline, extern "lean_task_spawn"]
 protected def spawn {α : Type u} (fn : Unit → α) (prio := Priority.default) : Task α :=
   ⟨fn ()⟩
 
 set_option linter.unusedVariables.funArgs false in
+/--
+`map f x` maps function `f` over the task `x`: that is, it constructs
+(and immediately launches) a new task which will wait for the value of `x` to
+be available and then calls `f` on the result.
+
+`prio`, if provided, is the priority of the task.
+-/
 @[noinline, extern "lean_task_map"]
 protected def map {α : Type u} {β : Type v} (f : α → β) (x : Task α) (prio := Priority.default) : Task β :=
   ⟨f x.get⟩
 
 set_option linter.unusedVariables.funArgs false in
+/--
+`bind x f` does a monad "bind" operation on the task `x` with function `f`:
+that is, it constructs (and immediately launches) a new task which will wait
+for the value of `x` to be available and then calls `f` on the result,
+resulting in a new task which is then run for a result.
+
+`prio`, if provided, is the priority of the task.
+-/
 @[noinline, extern "lean_task_bind"]
 protected def bind {α : Type u} {β : Type v} (x : Task α) (f : α → Task β) (prio := Priority.default) : Task β :=
   ⟨(f x.get).get⟩
 
 end Task
 
-/-- Some type that is not a scalar value in our runtime. -/
+/--
+`NonScalar` is a type that is not a scalar value in our runtime.
+It is used as a stand-in for an arbitrary boxed value to avoid excessive
+monomorphization, and it is only created using `unsafeCast`. It is somewhat
+analogous to C `void*` in usage, but the type itself is not special.
+-/
 structure NonScalar where
-  val : Nat
+  /-- You should not use this function -/ mk ::
+  /-- You should not use this function -/ val : Nat
 
-/-- Some type that is not a scalar value in our runtime and is universe polymorphic. -/
+/--
+`PNonScalar` is a type that is not a scalar value in our runtime.
+It is used as a stand-in for an arbitrary boxed value to avoid excessive
+monomorphization, and it is only created using `unsafeCast`. It is somewhat
+analogous to C `void*` in usage, but the type itself is not special.
+
+This is the universe-polymorphic version of `PNonScalar`; it is preferred to use
+`NonScalar` instead where applicable.
+-/
 inductive PNonScalar : Type u where
-  | mk (v : Nat) : PNonScalar
+  | /-- You should not use this function -/
+    mk (v : Nat) : PNonScalar
 
 @[simp] theorem Nat.add_zero (n : Nat) : n + 0 = n := rfl
 
@@ -181,17 +456,41 @@ theorem optParam_eq (α : Sort u) (default : α) : optParam α default = α := r
 
 /-! # Boolean operators -/
 
+/--
+`strictOr` is the same as `or`, but it does not use short-circuit evaluation semantics:
+both sides are evaluated, even if the first value is `true`.
+-/
 @[extern c inline "#1 || #2"] def strictOr  (b₁ b₂ : Bool) := b₁ || b₂
+
+/--
+`strictAnd` is the same as `and`, but it does not use short-circuit evaluation semantics:
+both sides are evaluated, even if the first value is `false`.
+-/
 @[extern c inline "#1 && #2"] def strictAnd (b₁ b₂ : Bool) := b₁ && b₂
 
+/--
+`x != y` is boolean not-equal. It is the negation of `x == y` which is supplied by
+the `BEq` typeclass.
+
+Unlike `x ≠ y` (which is notation for `Ne x y`), this is `Bool` valued instead of
+`Prop` valued. It is mainly intended for programming applications.
+-/
 @[inline] def bne {α : Type u} [BEq α] (a b : α) : Bool :=
   !(a == b)
 
-infix:50 " != " => bne
+@[inheritDoc] infix:50 " != " => bne
 
+/--
+`LawfulBEq α` is a typeclass which asserts that the `BEq α` implementation
+(which supplies the `a == b` notation) coincides with logical equality `a = b`.
+In other words, `a == b` implies `a = b`, and `a == a` is true.
+-/
 class LawfulBEq (α : Type u) [BEq α] : Prop where
-  eq_of_beq : {a b : α} → (a == b) = true → a = b
-  protected rfl : {a : α} → (a == a) = true
+  /-- If `a == b` evaluates to `true`, then `a` and `b` are equal in the logic. -/
+  eq_of_beq : {a b : α} → a == b → a = b
+  /-- `==` is reflexive, that is, `(a == a) = true`. -/
+  protected rfl : {a : α} → a == a
+
 export LawfulBEq (eq_of_beq)
 
 instance : LawfulBEq Bool where
@@ -208,7 +507,7 @@ instance : LawfulBEq String := inferInstance
 
 /-! # Logical connectives and equality -/
 
-def trivial : True := ⟨⟩
+@[inheritDoc True.intro] def trivial : True := ⟨⟩
 
 theorem mt {a b : Prop} (h₁ : a → b) (h₂ : ¬b) : ¬a :=
   fun ha => h₂ (h₁ ha)
@@ -223,9 +522,23 @@ theorem proofIrrel {a : Prop} (h₁ h₂ : a) : h₁ = h₂ := rfl
 
 theorem id.def {α : Sort u} (a : α) : id a = a := rfl
 
+/--
+If `h : α = β` is a proof of type equality, then `h.mp : α → β` is the induced
+"cast" operation, mapping elements of `α` to elements of `β`.
+
+You can prove theorems about the resulting element by induction on `h`, since
+`rfl.mp` is definitionally the identity function.
+-/
 @[macroInline] def Eq.mp {α β : Sort u} (h : α = β) (a : α) : β :=
   h ▸ a
 
+/--
+If `h : α = β` is a proof of type equality, then `h.mpr : β → α` is the induced
+"cast" operation in the reverse direction, mapping elements of `β` to elements of `α`.
+
+You can prove theorems about the resulting element by induction on `h`, since
+`rfl.mpr` is definitionally the identity function.
+-/
 @[macroInline] def Eq.mpr {α β : Sort u} (h : α = β) (b : β) : α :=
   h ▸ b
 
@@ -235,10 +548,14 @@ theorem Eq.substr {α : Sort u} {p : α → Prop} {a b : α} (h₁ : b = a) (h�
 theorem cast_eq {α : Sort u} (h : α = α) (a : α) : cast h a = a :=
   rfl
 
+/--
+`a ≠ b`, or `Ne a b` is defined as `¬ (a = b)` or `a = b → False`,
+and asserts that `a` and `b` are not equal.
+-/
 @[reducible] def Ne {α : Sort u} (a b : α) :=
   ¬(a = b)
 
-infix:50 " ≠ "  => Ne
+@[inheritDoc] infix:50 " ≠ "  => Ne
 
 section Ne
 variable {α : Sort u}
@@ -314,7 +631,7 @@ theorem heq_of_heq_of_eq (h₁ : HEq a b) (h₂ : b = b') : HEq a b' :=
 theorem heq_of_eq_of_heq (h₁ : a = a') (h₂ : HEq a' b) : HEq a b :=
   HEq.trans (heq_of_eq h₁) h₂
 
-def type_eq_of_heq (h : HEq a b) : α = β :=
+theorem type_eq_of_heq (h : HEq a b) : α = β :=
   h.rec (Eq.refl α)
 
 end
@@ -396,6 +713,11 @@ instance : Decidable False :=
 namespace Decidable
 variable {p q : Prop}
 
+/--
+Synonym for `dite` (dependent if-then-else). We can construct an element `q`
+(of any sort, not just a proposition) by cases on whether `p` is true or false,
+provided `p` is decidable.
+-/
 @[macroInline] def byCases {q : Sort u} [dec : Decidable p] (h1 : p → q) (h2 : ¬p → q) : q :=
   match dec with
   | isTrue h  => h1 h
@@ -425,13 +747,15 @@ end Decidable
 
 section
 variable {p q : Prop}
-@[inline] def  decidable_of_decidable_of_iff [Decidable p] (h : p ↔ q) : Decidable q :=
+/-- Transfer a decidability proof across an equivalence of propositions. -/
+@[inline] def decidable_of_decidable_of_iff [Decidable p] (h : p ↔ q) : Decidable q :=
   if hp : p then
     isTrue (Iff.mp h hp)
   else
     isFalse fun hq => absurd (Iff.mpr h hq) hp
 
-@[inline] def  decidable_of_decidable_of_eq [Decidable p] (h : p = q) : Decidable q :=
+/-- Transfer a decidability proof across an equality of propositions. -/
+@[inline] def decidable_of_decidable_of_eq [Decidable p] (h : p = q) : Decidable q :=
   decidable_of_decidable_of_iff (p := p) (h ▸ Iff.rfl)
 end
 
@@ -491,12 +815,13 @@ instance {c : Prop} {t : c → Prop} {e : ¬c → Prop} [dC : Decidable c] [dT :
   | isTrue hc  => dT hc
   | isFalse hc => dE hc
 
-/-- Auxiliary definitions for generating compact `noConfusion` for enumeration types -/
+/-- Auxiliary definition for generating compact `noConfusion` for enumeration types -/
 abbrev noConfusionTypeEnum {α : Sort u} {β : Sort v} [inst : DecidableEq β] (f : α → β) (P : Sort w) (x y : α) : Sort w :=
   (inst (f x) (f y)).casesOn
     (fun _ => P)
     (fun _ => P → P)
 
+/-- Auxiliary definition for generating compact `noConfusion` for enumeration types -/
 abbrev noConfusionEnum {α : Sort u} {β : Sort v} [inst : DecidableEq β] (f : α → β) {P : Sort w} {x y : α} (h : x = y) : noConfusionTypeEnum f P x y :=
   Decidable.casesOn
     (motive := fun (inst : Decidable (f x = f y)) => Decidable.casesOn (motive := fun _ => Sort w) inst (fun _ => P) (fun _ => P → P))
@@ -516,13 +841,24 @@ theorem nonempty_of_exists {α : Sort u} {p : α → Prop} : Exists (fun x => p 
 
 /-! # Subsingleton -/
 
+/--
+A "subsingleton" is a type with at most one element.
+In other words, it is either empty, or has a unique element.
+All propositions are subsingletons because of proof irrelevance, but some other types
+are subsingletons as well and they inherit many of the same properties as propositions.
+`Subsingleton α` is a typeclass, so it is usually used as an implicit argument and
+inferred by typeclass inference.
+-/
 class Subsingleton (α : Sort u) : Prop where
-  intro :: allEq : (a b : α) → a = b
+  /-- Construct a proof that `α` is a subsingleton by showing that any two elements are equal. -/
+  intro ::
+  /-- Any two elements of a subsingleton are equal. -/
+  allEq : (a b : α) → a = b
 
-protected def Subsingleton.elim {α : Sort u} [h : Subsingleton α] : (a b : α) → a = b :=
+protected theorem Subsingleton.elim {α : Sort u} [h : Subsingleton α] : (a b : α) → a = b :=
   h.allEq
 
-protected def Subsingleton.helim {α β : Sort u} [h₁ : Subsingleton α] (h₂ : α = β) (a : α) (b : β) : HEq a b := by
+protected theorem Subsingleton.helim {α β : Sort u} [h₁ : Subsingleton α] (h₂ : α = β) (a : α) (b : β) : HEq a b := by
   subst h₂
   apply heq_of_eq
   apply Subsingleton.elim
@@ -550,28 +886,58 @@ theorem recSubsingleton
   | isTrue h  => h₃ h
   | isFalse h => h₄ h
 
+/--
+An equivalence relation `~ : α → α → Prop` is a relation that is:
+
+* reflexive: `x ~ x`
+* symmetric: `x ~ y` implies `y ~ x`
+* transitive: `x ~ y` and `y ~ z` implies `x ~ z`
+
+Equality is an equivalence relation, and equivalence relations share many of
+the properties of equality. In particular, `Quot α r` is most well behaved
+when `r` is an equivalence relation, and in this case we use `Quotient` instead.
+-/
 structure Equivalence {α : Sort u} (r : α → α → Prop) : Prop where
+  /-- An equivalence relation is reflexive: `x ~ x` -/
   refl  : ∀ x, r x x
+  /-- An equivalence relation is symmetric: `x ~ y` implies `y ~ x` -/
   symm  : ∀ {x y}, r x y → r y x
+  /-- An equivalence relation is transitive: `x ~ y` and `y ~ z` implies `x ~ z` -/
   trans : ∀ {x y z}, r x y → r y z → r x z
 
+/-- The empty relation is the relation on `α` which is always `False`. -/
 def emptyRelation {α : Sort u} (_ _ : α) : Prop :=
   False
 
+/--
+`Subrelation q r` means that `q ⊆ r` or `∀ x y, q x y → r x y`.
+It is the analogue of the subset relation on relations.
+-/
 def Subrelation {α : Sort u} (q r : α → α → Prop) :=
   ∀ {x y}, q x y → r x y
 
+/--
+The inverse image of `r : β → β → Prop` by a function `α → β` is the relation
+`s : α → α → Prop` defined by `s a b = r (f a) (f b)`.
+-/
 def InvImage {α : Sort u} {β : Sort v} (r : β → β → Prop) (f : α → β) : α → α → Prop :=
   fun a₁ a₂ => r (f a₁) (f a₂)
 
+/--
+The transitive closure `r⁺` of a relation `r` is the smallest relation which is
+transitive and contains `r`. `r⁺ a z` if and only if there exists a sequence
+`a r b r ... r z` of length at least 1 connecting `a` to `z`.
+-/
 inductive TC {α : Sort u} (r : α → α → Prop) : α → α → Prop where
-  | base  : ∀ a b, r a b → TC r a b
-  | trans : ∀ a b c, TC r a b → TC r b c → TC r a c
+  | /-- If `r a b` then `r⁺ a b`. This is the base case of the transitive closure. -/
+    base  : ∀ a b, r a b → TC r a b
+  | /-- The transitive closure is transitive. -/
+    trans : ∀ a b c, TC r a b → TC r b c → TC r a c
 
 /-! # Subtype -/
 
 namespace Subtype
-def existsOfSubtype {α : Type u} {p : α → Prop} : { x // p x } → Exists (fun x => p x)
+theorem existsOfSubtype {α : Type u} {p : α → Prop} : { x // p x } → Exists (fun x => p x)
   | ⟨a, h⟩ => ⟨a, h⟩
 
 variable {α : Type u} {p : α → Prop}
@@ -655,6 +1021,10 @@ theorem Prod.lt_def [LT α] [LT β] (s t : α × β) : (s < t) = (s.1 < t.1 ∨ 
 theorem Prod.ext (p : α × β) : (p.1, p.2) = p := by
   cases p; rfl
 
+/--
+`Prod.map f g : α₁ × β₁ → α₂ × β₂` maps across a pair
+by applying `f` to the first component and `g` to the second.
+-/
 def Prod.map {α₁ : Type u₁} {α₂ : Type u₂} {β₁ : Type v₁} {β₂ : Type v₂}
     (f : α₁ → α₂) (g : β₁ → β₂) : α₁ × β₁ → α₂ × β₂
   | (a, b) => (f a, g b)
@@ -689,8 +1059,14 @@ instance : DecidableEq PUnit :=
 
 /-! # Setoid -/
 
+/--
+A setoid is a type with a distinguished equivalence relation, denoted `≈`.
+This is mainly used as input to the `Quotient` type constructor.
+-/
 class Setoid (α : Sort u) where
+  /-- `x ≈ y` is the distinguished equivalence relation of a setoid. -/
   r : α → α → Prop
+  /-- The relation `x ≈ y` is an equivalence relation. -/
   iseqv : Equivalence r
 
 instance {α : Sort u} [Setoid α] : HasEquiv α :=
@@ -714,6 +1090,40 @@ end Setoid
 
 /-! # Propositional extensionality -/
 
+/--
+The axiom of **propositional extensionality**. It asserts that if propositions
+`a` and `b` are logically equivalent (i.e. we can prove `a` from `b` and vice versa),
+then `a` and `b` are *equal*, meaning that we can replace `a` with `b` in all
+contexts.
+
+For simple expressions like `a ∧ c ∨ d → e` we can prove that because all the logical
+connectives respect logical equivalence, we can replace `a` with `b` in this expression
+without using `propext`. However, for higher order expressions like `P a` where
+`P : Prop → Prop` is unknown, or indeed for `a = b` itself, we cannot replace `a` with `b`
+without an axiom which says exactly this.
+
+This is a relatively uncontroversial axiom, which is intuitionistically valid.
+It does however block computation when using `#reduce` to reduce proofs directly
+(which is not recommended), meaning that canonicity,
+the property that all closed terms of type `Nat` normalize to numerals,
+fails to hold when this (or any) axiom is used:
+```
+set_option pp.proofs true
+
+def foo : Nat := by
+  have : (True → True) ↔ True := ⟨λ _ => trivial, λ _ _ => trivial⟩
+  have := propext this ▸ (2 : Nat)
+  exact this
+
+#reduce foo
+-- propext { mp := fun x x => True.intro, mpr := fun x => True.intro } ▸ 2
+
+#eval foo -- 2
+```
+`#eval` can evaluate it to a numeral because the compiler erases casts and
+does not evaluate proofs, so `propext`, whose return type is a proposition,
+can never block it.
+-/
 axiom propext {a b : Prop} : (a ↔ b) → a = b
 
 theorem Eq.propIntro {a b : Prop} (h₁ : a → b) (h₂ : b → a) : a = b :=
@@ -751,6 +1161,36 @@ theorem Iff.subst {a b : Prop} {p : Prop → Prop} (h₁ : a ↔ b) (h₂ : p a)
   Eq.subst (propext h₁) h₂
 
 namespace Quot
+/--
+The **quotient axiom**, or at least the nontrivial part of the quotient
+axiomatization. Quotient types are introduced by the `init_quot` command
+in `Init.Prelude` which introduces the axioms:
+
+```
+opaque Quot {α : Sort u} (r : α → α → Prop) : Sort u
+
+opaque Quot.mk {α : Sort u} (r : α → α → Prop) (a : α) : Quot r
+
+opaque Quot.lift {α : Sort u} {r : α → α → Prop} {β : Sort v} (f : α → β) :
+  (∀ a b : α, r a b → f a = f b) → Quot r → β
+
+opaque Quot.ind {α : Sort u} {r : α → α → Prop} {β : Quot r → Prop} :
+  (∀ a : α, β (Quot.mk r a)) → ∀ q : Quot r, β q
+```
+All of these axioms are true if we assume `Quot α r = α` and `Quot.mk` and
+`Quot.lift` are identity functions, so they do not add much. However this axiom
+cannot be explained in that way (it is false for that interpretation), so the
+real power of quotient types come from this axiom.
+
+It says that the quotient by `r` maps elements which are related by `r` to equal
+values in the quotient. Together with `Quot.lift` which says that functions
+which respect `r` can be lifted to functions on the quotient, we can deduce that
+`Quot α r` exactly consists of the equivalence classes with respect to `r`.
+
+It is important to note that `r` need not be an equivalence relation in this axiom.
+When `r` is not an equivalence relation, we are actually taking a quotient with
+respect to the equivalence relation generated by `r`.
+-/
 axiom sound : ∀ {α : Sort u} {r : α → α → Prop} {a b : α}, r a b → Quot.mk r a = Quot.mk r b
 
 protected theorem liftBeta {α : Sort u} {r : α → α → Prop} {β : Sort v}
@@ -766,7 +1206,12 @@ protected theorem indBeta {α : Sort u} {r : α → α → Prop} {motive : Quot 
     : (ind p (Quot.mk r a) : motive (Quot.mk r a)) = p a :=
   rfl
 
-protected abbrev liftOn {α : Sort u} {β : Sort v} {r : α → α → Prop} (q : Quot r) (f : α → β) (c : (a b : α) → r a b → f a = f b) : β :=
+/--
+`Quot.liftOn q f h` is the same as `Quot.lift f h q`. It just reorders
+the argument `q : Quot r` to be first.
+-/
+protected abbrev liftOn {α : Sort u} {β : Sort v} {r : α → α → Prop}
+  (q : Quot r) (f : α → β) (c : (a b : α) → r a b → f a = f b) : β :=
   lift f c q
 
 @[elabAsElim]
@@ -784,6 +1229,7 @@ variable {α : Sort u}
 variable {r : α → α → Prop}
 variable {motive : Quot r → Sort v}
 
+/-- Auxiliary definition for `Quot.rec`. -/
 @[reducible, macroInline]
 protected def indep (f : (a : α) → motive (Quot.mk r a)) (a : α) : PSigma motive :=
   ⟨Quot.mk r a, f a⟩
@@ -802,19 +1248,31 @@ protected theorem liftIndepPr1
  induction q using Quot.ind
  exact rfl
 
+/--
+Dependent recursion principle for `Quot`. This constructor can be tricky to use,
+so you should consider the simpler versions if they apply:
+* `Quot.lift`, for nondependent functions
+* `Quot.ind`, for theorems / proofs of propositions about quotients
+* `Quot.recOnSubsingleton`, when the target type is a `Subsingleton`
+* `Quot.hrecOn`, which uses `HEq (f a) (f b)` instead of a `sound p ▸ f a = f b` assummption
+-/
 protected abbrev rec
     (f : (a : α) → motive (Quot.mk r a))
     (h : (a b : α) → (p : r a b) → Eq.ndrec (f a) (sound p) = f b)
     (q : Quot r) : motive q :=
   Eq.ndrecOn (Quot.liftIndepPr1 f h q) ((lift (Quot.indep f) (Quot.indepCoherent f h) q).2)
 
-protected abbrev recOn
+@[inheritDoc Quot.rec] protected abbrev recOn
     (q : Quot r)
     (f : (a : α) → motive (Quot.mk r a))
     (h : (a b : α) → (p : r a b) → Eq.ndrec (f a) (sound p) = f b)
     : motive q :=
  q.rec f h
 
+/--
+Dependent induction principle for a quotient, when the target type is a `Subsingleton`.
+In this case the quotient's side condition is trivial so any function can be lifted.
+-/
 protected abbrev recOnSubsingleton
     [h : (a : α) → Subsingleton (motive (Quot.mk r a))]
     (q : Quot r)
@@ -824,6 +1282,11 @@ protected abbrev recOnSubsingleton
   apply f
   apply Subsingleton.elim
 
+/--
+Heterogeneous dependent recursion principle for a quotient.
+This may be easier to work with since it uses `HEq` instead of
+an `Eq.ndrec` in the hypothesis.
+-/
 protected abbrev hrecOn
     (q : Quot r)
     (f : (a : α) → motive (Quot.mk r a))
@@ -837,27 +1300,49 @@ end
 end Quot
 
 set_option linter.unusedVariables.funArgs false in
+/--
+`Quotient α s` is the same as `Quot α r`, but it is specialized to a setoid `s`
+(that is, an equivalence relation) instead of an arbitrary relation.
+Prefer `Quotient` over `Quot` if your relation is actually an equivalence relation.
+-/
 def Quotient {α : Sort u} (s : Setoid α) :=
   @Quot α Setoid.r
 
 namespace Quotient
 
+/-- The canonical quotient map into a `Quotient`. -/
 @[inline]
 protected def mk {α : Sort u} (s : Setoid α) (a : α) : Quotient s :=
   Quot.mk Setoid.r a
 
+/--
+The canonical quotient map into a `Quotient`.
+(This synthesizes the setoid by typeclass inference.)
+-/
 protected def mk' {α : Sort u} [s : Setoid α] (a : α) : Quotient s :=
   Quotient.mk s a
 
+/--
+The analogue of `Quot.sound`: If `a` and `b` are related by the equivalence relation,
+then they have equal equivalence classes.
+-/
 def sound {α : Sort u} {s : Setoid α} {a b : α} : a ≈ b → Quotient.mk s a = Quotient.mk s b :=
   Quot.sound
 
+/--
+The analogue of `Quot.lift`: if `f : α → β` respects the equivalence relation `≈`,
+then it lifts to a function on `Quotient s` such that `lift f h (mk a) = f a`.
+-/
 protected abbrev lift {α : Sort u} {β : Sort v} {s : Setoid α} (f : α → β) : ((a b : α) → a ≈ b → f a = f b) → Quotient s → β :=
   Quot.lift f
 
 protected theorem ind {α : Sort u} {s : Setoid α} {motive : Quotient s → Prop} : ((a : α) → motive (Quotient.mk s a)) → (q : Quot Setoid.r) → motive q :=
   Quot.ind
 
+/--
+The analogue of `Quot.liftOn`: if `f : α → β` respects the equivalence relation `≈`,
+then it lifts to a function on `Quotient s` such that `lift (mk a) f h = f a`.
+-/
 protected abbrev liftOn {α : Sort u} {β : Sort v} {s : Setoid α} (q : Quotient s) (f : α → β) (c : (a b : α) → a ≈ b → f a = f b) : β :=
   Quot.liftOn q f c
 
@@ -876,6 +1361,7 @@ variable {α : Sort u}
 variable {s : Setoid α}
 variable {motive : Quotient s → Sort v}
 
+/-- The analogue of `Quot.rec` for `Quotient`. See `Quot.rec`. -/
 @[inline, elabAsElim]
 protected def rec
     (f : (a : α) → motive (Quotient.mk s a))
@@ -884,6 +1370,7 @@ protected def rec
     : motive q :=
   Quot.rec f h q
 
+/-- The analogue of `Quot.recOn` for `Quotient`. See `Quot.recOn`. -/
 @[elabAsElim]
 protected abbrev recOn
     (q : Quotient s)
@@ -892,6 +1379,7 @@ protected abbrev recOn
     : motive q :=
   Quot.recOn q f h
 
+/-- The analogue of `Quot.recOnSubsingleton` for `Quotient`. See `Quot.recOnSubsingleton`. -/
 @[elabAsElim]
 protected abbrev recOnSubsingleton
     [h : (a : α) → Subsingleton (motive (Quotient.mk s a))]
@@ -900,6 +1388,7 @@ protected abbrev recOnSubsingleton
     : motive q :=
   Quot.recOnSubsingleton (h := h) q f
 
+/-- The analogue of `Quot.hrecOn` for `Quotient`. See `Quot.hrecOn`. -/
 @[elabAsElim]
 protected abbrev hrecOn
     (q : Quotient s)
@@ -914,6 +1403,7 @@ universe uA uB uC
 variable {α : Sort uA} {β : Sort uB} {φ : Sort uC}
 variable {s₁ : Setoid α} {s₂ : Setoid β}
 
+/-- Lift a binary function to a quotient on both arguments. -/
 protected abbrev lift₂
     (f : α → β → φ)
     (c : (a₁ : α) → (b₁ : β) → (a₂ : α) → (b₂ : β) → a₁ ≈ a₂ → b₁ ≈ b₂ → f a₁ b₁ = f a₂ b₂)
@@ -924,6 +1414,7 @@ protected abbrev lift₂
   induction q₂ using Quotient.ind
   apply c; assumption; apply Setoid.refl
 
+/-- Lift a binary function to a quotient on both arguments. -/
 protected abbrev liftOn₂
     (q₁ : Quotient s₁)
     (q₂ : Quotient s₂)
@@ -998,6 +1489,7 @@ universe uA uB uC
 variable {α : Sort uA} {β : Sort uB}
 variable {s₁ : Setoid α} {s₂ : Setoid β}
 
+/-- Lift a binary function to a quotient on both arguments. -/
 @[elabAsElim]
 protected abbrev recOnSubsingleton₂
     {motive : Quotient s₁ → Quotient s₂ → Sort uC}
@@ -1031,29 +1523,56 @@ instance {α : Sort u} {s : Setoid α} [d : ∀ (a b : α), Decidable (a ≈ b)]
 
 /-! # Function extensionality -/
 
-theorem funext {α : Sort u} {β : α → Sort v} {f₁ f₂ : (x : α) → β x}
-    (h : ∀ x, f₁ x = f₂ x) : f₁ = f₂ := by
-  let eqv (f₁ f₂ : (x : α) → β x) := ∀ x, f₁ x = f₂ x
+/--
+**Function extensionality** is the statement that if two functions take equal values
+every point, then the functions themselves are equal: `(∀ x, f x = g x) → f = g`.
+It is called "extensionality" because it talks about how to prove two objects are equal
+based on the properties of the object (compare with set extensionality,
+which is `(∀ x, x ∈ s ↔ x ∈ t) → s = t`).
+
+This is often an axiom in dependent type theory systems, because it cannot be proved
+from the core logic alone. However in lean's type theory this follows from the existence
+of quotient types (note the `Quot.sound` in the proof, as well as the `show` line
+which makes use of the definitional equality `Quot.lift f h (Quot.mk x) = f x`).
+-/
+theorem funext {α : Sort u} {β : α → Sort v} {f g : (x : α) → β x}
+    (h : ∀ x, f x = g x) : f = g := by
+  let eqv (f g : (x : α) → β x) := ∀ x, f x = g x
   let extfunApp (f : Quot eqv) (x : α) : β x :=
     Quot.liftOn f
       (fun (f : ∀ (x : α), β x) => f x)
       (fun _ _ h => h x)
-  show extfunApp (Quot.mk eqv f₁) = extfunApp (Quot.mk eqv f₂)
+  show extfunApp (Quot.mk eqv f) = extfunApp (Quot.mk eqv g)
   exact congrArg extfunApp (Quot.sound h)
 
 instance {α : Sort u} {β : α → Sort v} [∀ a, Subsingleton (β a)] : Subsingleton (∀ a, β a) where
-  allEq f₁ f₂ :=
-    funext (fun a => Subsingleton.elim (f₁ a) (f₂ a))
+  allEq f g := funext fun a => Subsingleton.elim (f a) (g a)
 
 /-! # Squash -/
 
+/--
+`Squash α` is the quotient of `α` by the always true relation.
+It is empty if `α` is empty, otherwise it is a singleton.
+(Thus it is unconditionally a `Subsingleton`.)
+It is the "universal `Subsingleton`" mapped from `α`.
+
+It is similar to `Nonempty α`, which has the same properties, but unlike
+`Nonempty` this is a `Type u`, that is, it is "data", and the compiler
+represents an element of `Squash α` the same as `α` itself
+(as compared to `Nonempty α`, whose elements are represented by a dummy value).
+
+`Squash.lift` will extract a value in any subsingleton `β` from a function on `α`,
+while `Nonempty.rec` can only do the same when `β` is a proposition.
+-/
 def Squash (α : Type u) := Quot (fun (_ _ : α) => True)
 
+/-- The canonical quotient map into `Squash α`. -/
 def Squash.mk {α : Type u} (x : α) : Squash α := Quot.mk _ x
 
 theorem Squash.ind {α : Type u} {motive : Squash α → Prop} (h : ∀ (a : α), motive (Squash.mk a)) : ∀ (q : Squash α), motive q :=
   Quot.ind h
 
+/-- If `β` is a subsingleton, then a function `α → β` lifts to `Squash α → β`. -/
 @[inline] def Squash.lift {α β} [Subsingleton β] (s : Squash α) (f : α → β) : β :=
   Quot.lift f (fun _ _ _ => Subsingleton.elim _ _) s
 
@@ -1066,55 +1585,106 @@ instance : Subsingleton (Squash α) where
 
 /-! # Relations -/
 
+/--
+`Antisymm (·≤·)` says that `(·≤·)` is antisymmetric, that is, `a ≤ b → b ≤ a → a = b`.
+-/
 class Antisymm {α : Sort u} (r : α → α → Prop) where
+  /-- An antisymmetric relation `(·≤·)` satisfies `a ≤ b → b ≤ a → a = b`. -/
   antisymm {a b : α} : r a b → r b a → a = b
 
 namespace Lean
 /-! # Kernel reduction hints -/
 
 /--
-  When the kernel tries to reduce a term `Lean.reduceBool c`, it will invoke the Lean interpreter to evaluate `c`.
-  The kernel will not use the interpreter if `c` is not a constant.
-  This feature is useful for performing proofs by reflection.
+When the kernel tries to reduce a term `Lean.reduceBool c`, it will invoke the Lean interpreter to evaluate `c`.
+The kernel will not use the interpreter if `c` is not a constant.
+This feature is useful for performing proofs by reflection.
 
-  Remark: the Lean frontend allows terms of the from `Lean.reduceBool t` where `t` is a term not containing
-  free variables. The frontend automatically declares a fresh auxiliary constant `c` and replaces the term with
-  `Lean.reduceBool c`. The main motivation is that the code for `t` will be pre-compiled.
+Remark: the Lean frontend allows terms of the from `Lean.reduceBool t` where `t` is a term not containing
+free variables. The frontend automatically declares a fresh auxiliary constant `c` and replaces the term with
+`Lean.reduceBool c`. The main motivation is that the code for `t` will be pre-compiled.
 
-  Warning: by using this feature, the Lean compiler and interpreter become part of your trusted code base.
-  This is extra 30k lines of code. More importantly, you will probably not be able to check your developement using
-  external type checkers (e.g., Trepplein) that do not implement this feature.
-  Keep in mind that if you are using Lean as programming language, you are already trusting the Lean compiler and interpreter.
-  So, you are mainly losing the capability of type checking your developement using external checkers.
+Warning: by using this feature, the Lean compiler and interpreter become part of your trusted code base.
+This is extra 30k lines of code. More importantly, you will probably not be able to check your development using
+external type checkers (e.g., Trepplein) that do not implement this feature.
+Keep in mind that if you are using Lean as programming language, you are already trusting the Lean compiler and interpreter.
+So, you are mainly losing the capability of type checking your development using external checkers.
 
-  Recall that the compiler trusts the correctness of all `[implementedBy ...]` and `[extern ...]` annotations.
-  If an extern function is executed, then the trusted code base will also include the implementation of the associated
-  foreign function.
+Recall that the compiler trusts the correctness of all `[implementedBy ...]` and `[extern ...]` annotations.
+If an extern function is executed, then the trusted code base will also include the implementation of the associated
+foreign function.
 -/
 opaque reduceBool (b : Bool) : Bool := b
 
 /--
-  Similar to `Lean.reduceBool` for closed `Nat` terms.
+Similar to `Lean.reduceBool` for closed `Nat` terms.
 
-  Remark: we do not have plans for supporting a generic `reduceValue {α} (a : α) : α := a`.
-  The main issue is that it is non-trivial to convert an arbitrary runtime object back into a Lean expression.
-  We believe `Lean.reduceBool` enables most interesting applications (e.g., proof by reflection). -/
+Remark: we do not have plans for supporting a generic `reduceValue {α} (a : α) : α := a`.
+The main issue is that it is non-trivial to convert an arbitrary runtime object back into a Lean expression.
+We believe `Lean.reduceBool` enables most interesting applications (e.g., proof by reflection).
+-/
 opaque reduceNat (n : Nat) : Nat := n
 
-axiom ofReduceBool (a b : Bool) (h : reduceBool a = b) : a = b
-axiom ofReduceNat (a b : Nat) (h : reduceNat a = b)    : a = b
+/--
+The axiom `ofReduceBool` is used to perform proofs by reflection. See `reduceBool`.
 
+This axiom is usually not used directly, because it has some syntactic restrictions.
+Instead, the `native_decide` tactic can be used to prove any proposition whose
+decidability instance can be evaluated to `true` using the lean compiler / interpreter.
+
+Warning: by using this feature, the Lean compiler and interpreter become part of your trusted code base.
+This is extra 30k lines of code. More importantly, you will probably not be able to check your development using
+external type checkers (e.g., Trepplein) that do not implement this feature.
+Keep in mind that if you are using Lean as programming language, you are already trusting the Lean compiler and interpreter.
+So, you are mainly losing the capability of type checking your development using external checkers.
+-/
+axiom ofReduceBool (a b : Bool) (h : reduceBool a = b) : a = b
+
+/--
+The axiom `ofReduceNat` is used to perform proofs by reflection. See `reduceBool`.
+
+Warning: by using this feature, the Lean compiler and interpreter become part of your trusted code base.
+This is extra 30k lines of code. More importantly, you will probably not be able to check your development using
+external type checkers (e.g., Trepplein) that do not implement this feature.
+Keep in mind that if you are using Lean as programming language, you are already trusting the Lean compiler and interpreter.
+So, you are mainly losing the capability of type checking your development using external checkers.
+-/
+axiom ofReduceNat (a b : Nat) (h : reduceNat a = b) : a = b
+
+/--
+`IsAssociative op` says that `op` is an associative operation,
+i.e. `(a ∘ b) ∘ c = a ∘ (b ∘ c)`. It is used by the `ac_rfl` tactic.
+-/
 class IsAssociative {α : Sort u} (op : α → α → α) where
+  /-- An associative operation satisfies `(a ∘ b) ∘ c = a ∘ (b ∘ c)`. -/
   assoc : (a b c : α) → op (op a b) c = op a (op b c)
 
+/--
+`IsCommutative op` says that `op` is a commutative operation,
+i.e. `a ∘ b = b ∘ a`. It is used by the `ac_rfl` tactic.
+-/
 class IsCommutative {α : Sort u} (op : α → α → α) where
+  /-- A commutative operation satisfies `a ∘ b = b ∘ a`. -/
   comm : (a b : α) → op a b = op b a
 
+/--
+`IsIdempotent op` says that `op` is an idempotent operation,
+i.e. `a ∘ a = a`. It is used by the `ac_rfl` tactic
+(which also simplifies up to idempotence when available).
+-/
 class IsIdempotent {α : Sort u} (op : α → α → α) where
+  /-- An idempotent operation satisfies `a ∘ a = a`. -/
   idempotent : (x : α) → op x x = x
 
+/--
+`IsNeutral op e` says that `e` is a neutral operation for `op`,
+i.e. `a ∘ e = a = e ∘ a`. It is used by the `ac_rfl` tactic
+(which also simplifies neutral elements when available).
+-/
 class IsNeutral {α : Sort u} (op : α → α → α) (neutral : α) where
+  /-- A neutral element can be cancelled on the left: `e ∘ a = a`. -/
   left_neutral : (a : α) → op neutral a = a
+  /-- A neutral element can be cancelled on the right: `a ∘ e = a`. -/
   right_neutral : (a : α) → op a neutral = a
 
 end Lean
